refactor

Cslib/Foundations/Logic/Model.lean
@@ -17,12 +17,11 @@ public import Cslib.Logics.HML.Basic
 This file is a **draft** proposal for how CSLib might factor out useful semantic concepts across
 different logics, in order to share notation and basic results. Some concepts we aim to unify are:
 
-- A satisfaction relation: `Models α β` (resp. `ParamModels α β`) indicates that a "model" `M : β`
-carries a satisfaction relation `Satisfies : β → α → Prop` over the "proposition" type α (resp.
-a local `SatisfiesAt : (b : β) → (Param b) → α → Prop`). Examples are `Modal.Satisfies` and
-`HML.Satisfies`.
+- A satisfaction relation: `HasEntails Model Formula` indicates that a "model" `M : Model`
+carries a satisfaction relation `Entails : Model → Formula → Prop` over the "proposition" type
+`Formula`. Examples are `Modal.Satisfies` and `HML.Satisfies`.
 - Soundness and completeness wrt an inference system.
-- The `theory` associated to a parameter, and the `logic` associated to a class of models. This
+- The `theory` associated to a single model, and the `logic` associated to a set of models. This
 captures `HML.theory`, `Modal.theory` and `Modal.logic`.
 
 Further developments could include relating different models of a given logic, models of
@@ -33,117 +32,112 @@ public section
 
 namespace Cslib.Logic
 
-/-- Objects of type `β` carry a forcing relation with the proposition type `α`. -/
-class Models (α : outParam Type*) (β : Type*) where
-  /-- `Satisfies b a` has the intended semantics "`a` is valid in the model `b`". -/
-  Satisfies : β → α → Prop
+/-- Objects of type `Model` carry a forcing relation with the proposition type `Formula`. -/
+class HasEntails (Model : Type*) (Formula : outParam Type*) where
+  /-- `Entails b a` has the intended semantics "`a` is valid in the model `b`". -/
+  Entails : Model → Formula → Prop
 
-scoped notation "⊨[" b "] " a => Models.Satisfies b a
-
-/-- Objects of type `β` carry a forcing relation worlds of type `γ` and the proposition type `α`. -/
-class ParamModels (α : outParam Type*) (β : Type*) where
-  Param : β → Type*
-  /-- Forcing relation associated to each parameter. -/
-  SatisfiesAt (b : β) : (Param b) → α → Prop
-
-scoped notation w " ⊨[" b "] " a => ParamModels.SatisfiesAt b w a
-
-instance ParamModels.toModels {α β : Type*} [ParamModels α β] : Models α β where
-  Satisfies M A := ∀ w : ParamModels.Param M, w ⊨[M] A
+scoped notation M " ⊨ " A => HasEntails.Entails M A
 
 /-- Bundled interpretation function. -/
-class HasInterp (α : outParam Type*) (β : Type*) where
+class HasInterp (Model : Type*) (Formula : outParam Type*) where
   /-- Type carrying interpretation. -/
-  Ground : β → Type*
+  Ground : Model → Type*
   /-- Interpret a proposition in a model. -/
-  interp : (b : β) → α → Ground b
+  interp : (M : Model) → Formula → Ground M
 
 /-- An `InterpModel` consists of an interpretation function, and a set specifying which
   interpretations are considered valid. -/
-class InterpModels (α : outParam (Type*)) (β : Type*) extends HasInterp α β where
+class HasInterpEntails (Model : Type*) (Formula : outParam Type*) extends
+    HasInterp Model Formula where
   /-- The set of valid interpretations. -/
-  filter (b : β) : Set (Ground b)
+  filter (M : Model) : Set (Ground M)
 
-instance InterpModels.instModels {α β : Type*} [InterpModels α β] : Models α β where
-  Satisfies b a := HasInterp.interp b a ∈ filter b
+instance HasInterpEntails.instHasEntails {Model Formula : Type*}
+    [HasInterpEntails Model Formula] : HasEntails Model Formula where
+  Entails b a := HasInterp.interp b a ∈ filter b
 
 namespace HasInterp
 
-class AlgebraicAnd (α β : Type*) [HasInterp α β] [HasAnd α] [∀ b : β, Min (Ground b)] where
-  interp_and_eq (M : β) (x y : α) : interp M (x ∧ y) = interp M x ⊓ interp M y
+class AlgebraicAnd (Model Formula : Type*) [HasInterp Model Formula] [HasAnd Formula]
+    [∀ M : Model, Min (Ground M)] where
+  interp_and_eq (M : Model) (x y : Formula) : interp M (x ∧ y) = interp M x ⊓ interp M y
 
-class AlgebraicOr (α β : Type*) [HasInterp α β] [HasOr α] [∀ b : β, Max (Ground b)] where
-  interp_or_eq (M : β) (x y : α) : interp M (x ∨ y) = interp M x ⊔ interp M y
+class AlgebraicOr (Model Formula : Type*) [HasInterp Model Formula] [HasOr Formula]
+    [∀ M : Model, Max (Ground M)] where
+  interp_or_eq (M : Model) (x y : Formula) : interp M (x ∨ y) = interp M x ⊔ interp M y
 
-class AlgebraicImpl (α β : Type*) [HasInterp α β] [HasImpl α] [∀ b : β, HImp (Ground b)] where
-  interp_impl_eq (M : β) (x y : α) : interp M (x → y) = interp M x ⇨ interp M y
+class AlgebraicImpl (Model Formula : Type*) [HasInterp Model Formula] [HasImpl Formula]
+    [∀ M : Model, HImp (Ground M)] where
+  interp_impl_eq (M : Model) (x y : Formula) : interp M (x → y) = interp M x ⇨ interp M y
 
-class AlgebraicNot (α β : Type*) [HasInterp α β] [HasNot α] [∀ b : β, Compl (Ground b)] where
-  interp_not_eq (M : β) (x y : α) : interp M (¬ x) = (interp M x)ᶜ
+class AlgebraicNot (Model Formula : Type*) [HasInterp Model Formula] [HasNot Formula]
+    [∀ M : Model, Compl (Ground M)] where
+  interp_not_eq (M : Model) (x y : Formula) : interp M (¬ x) = (interp M x)ᶜ
 
 end HasInterp
 
-open Models ParamModels InferenceSystem
+open HasEntails InferenceSystem
 
-variable {α β T} [Models α β] [InferenceSystem T α]
+variable {Model Formula T} [HasEntails Model Formula] [InferenceSystem T Formula]
 
-def SoundFor (α β T) [Models α β] [InferenceSystem T α] (S : Set β) : Prop :=
-  ∀ (A : α), DerivableIn T A → ∀ M ∈ S, ⊨[M] A
+def SoundFor (Model Formula T) [HasEntails Model Formula] [InferenceSystem T Formula]
+    (S : Set Model) : Prop := ∀ (A : Formula), DerivableIn T A → ∀ M ∈ S, M ⊨ A
 
-lemma SoundFor.subset {S S' : Set β} (hS : S ⊆ S') : SoundFor α β T S' → SoundFor α β T S :=
-  fun h A hA M hM => h A hA M (hS hM)
+lemma SoundFor.subset {S S' : Set Model} (hS : S ⊆ S') :
+    SoundFor Model Formula T S' → SoundFor Model Formula T S := fun h A hA M hM => h A hA M (hS hM)
 
-def CompleteFor (α β T : Type*) [Models α β] [InferenceSystem T α] (S : Set β) : Prop :=
-  ∀ A : α, (∀ M ∈ S, ⊨[M] A) → DerivableIn T A
+def CompleteFor (Model Formula T : Type*) [HasEntails Model Formula] [InferenceSystem T Formula]
+    (S : Set Model) : Prop := ∀ A : Formula, (∀ M ∈ S, M ⊨ A) → DerivableIn T A
 
-lemma CompleteFor.supset {S S' : Set β} (hS : S ⊆ S') :
-    CompleteFor α β T S → CompleteFor α β T S' := fun h A hA => h A (fun M hM => hA M (hS hM))
+lemma CompleteFor.supset {S S' : Set Model} (hS : S ⊆ S') :
+    CompleteFor Model Formula T S → CompleteFor Model Formula T S' :=
+  fun h A hA => h A (fun M hM => hA M (hS hM))
 
-def IsCompleteModel (α β T) [Models α β] [InferenceSystem T α] (M : β) : Prop :=
-  ∀ (A : α), (⊨[M] A) → DerivableIn T A
+def IsCompleteModel (Model Formula T) [HasEntails Model Formula] [InferenceSystem T Formula]
+    (M : Model) : Prop := ∀ (A : Formula), (M ⊨ A) → DerivableIn T A
 
-def ParamModels.theory {α β : Type*} [ParamModels α β] {M : β} (w : Param M) : Set α :=
-  {A : α | w ⊨[M] A}
+def HasEntails.theory {Model Formula : Type*} [HasEntails Model Formula] (M : Model) :
+    Set Formula := {A : Formula | M ⊨ A}
 
-def Models.logic {α β : Type*} [Models α β] (S : Set β) : Set α := {A | ∀ b ∈ S, ⊨[b] A}
+def HasEntails.logic {Model Formula : Type*} [HasEntails Model Formula] (S : Set Model) :
+    Set Formula := {A | ∀ M ∈ S, M ⊨ A}
 
-structure BundledModel (Atom : Type*) where
-  World : Type*
-  model : Modal.Model World Atom
+/-! ### Modal logic
 
-def Modal.Model.toBundledModel {World Atom : Type*} (M : Modal.Model World Atom) :
-  BundledModel Atom := {World := World, model := M}
+NB: we define entailment for pairs `(M, w)` of `M : Modal.Model World Atom` and a world `w`.
+-/
 
-/-- Instance using the bundled design. -/
-instance {Atom : Type*} : ParamModels (Modal.Proposition Atom) (BundledModel Atom) where
-  Param M := M.World
-  SatisfiesAt M w A := Modal.Satisfies M.model w A
-
-example {World Atom : Type*} (S : Set (Modal.Model World Atom)) :
-    Modal.logic S = Models.logic (Modal.Model.toBundledModel '' S) := by
-  simp [Models.logic]
-  rfl
-
-example {World Atom : Type*} (m : Modal.Model World Atom) (w : World) :
-    Modal.theory m w = ParamModels.theory (M := m.toBundledModel) w := rfl
+section Modal
 
 /-- Instance for "local forcing" (ie at the specific world) using unbundled design. -/
 instance {Atom World : Type*} :
-    Models (Modal.Proposition Atom) (Modal.Model World Atom × World) where
-  Satisfies M A := Modal.Satisfies M.1 M.2 A
+    HasEntails (Modal.Model World Atom × World) (Modal.Proposition Atom) where
+  Entails M A := Modal.Satisfies M.1 M.2 A
 
 /-- Global forcing in the unbundled design. -/
 instance {Atom World : Type*} :
-    Models (Modal.Proposition Atom) (Modal.Model World Atom) where
-  Satisfies M A := ∀ w : World, Modal.Satisfies M w A
+    HasEntails (Modal.Model World Atom) (Modal.Proposition Atom) where
+  Entails M A := ∀ w : World, Modal.Satisfies M w A
+
+example {World Atom : Type*} (M : Modal.Model World Atom) (w : World) (A : Modal.Proposition Atom) :
+    Modal.Satisfies M w A ↔ (M, w) ⊨ A := by rfl
+
+example {World Atom : Type*} (M : Modal.Model World Atom) (A : Modal.Proposition Atom) :
+    A.valid {M} ↔ M ⊨ A := by simp [Entails]; rfl
 
 example {World Atom : Type*} (M : Modal.Model World Atom) (w : World) :
-    Modal.theory M w = Models.logic {(M, w)} := by
-  simp [Modal.theory, logic]
-  rfl
+    Modal.theory M w = HasEntails.theory (M, w) := by rfl
 
 example {World Atom : Type*} (S : Set (Modal.Model World Atom)) :
-    Modal.logic S = Models.logic S := rfl
+    Modal.logic S = HasEntails.logic S := rfl
+
+end Modal
+
+/-! ### Propositional logic
+
+Examples for interpretation-style models of propositional logic.
+-/
 
 namespace PL
 
@@ -167,31 +161,31 @@ def HeytingModel.interp (M : HeytingModel Atom) : Proposition Atom → M.H
   | Proposition.or A B => M.interp A ⊔ M.interp B
   | Proposition.impl A B => M.interp A ⇨ M.interp B
 
-instance : InterpModels (Proposition Atom) (HeytingModel Atom) where
+instance : HasInterpEntails (HeytingModel Atom) (Proposition Atom) where
   Ground M := M.H
   interp := HeytingModel.interp
   filter _ := {⊤}
 
 instance (M : HeytingModel Atom) : GeneralizedHeytingAlgebra (HasInterp.Ground M) := M.inst
 
-instance : HasInterp.AlgebraicAnd (Proposition Atom) (HeytingModel Atom) where
+instance : HasInterp.AlgebraicAnd (HeytingModel Atom) (Proposition Atom) where
   interp_and_eq _ _ _ := rfl
 
-instance : HasInterp.AlgebraicOr (Proposition Atom) (HeytingModel Atom) where
+instance : HasInterp.AlgebraicOr (HeytingModel Atom) (Proposition Atom) where
   interp_or_eq _ _ _ := rfl
 
-instance : HasInterp.AlgebraicImpl (Proposition Atom) (HeytingModel Atom) where
+instance : HasInterp.AlgebraicImpl (HeytingModel Atom) (Proposition Atom) where
   interp_impl_eq _ _ _ := rfl
 
 theorem HeytingModel.sound [DecidableEq Atom] {T : Theory Atom} :
-    SoundFor (Proposition Atom) (HeytingModel Atom) T {M | ∀ A ∈ T, interp M A = ⊤} :=
+    SoundFor (HeytingModel Atom) (Proposition Atom) T {M | ∀ A ∈ T, interp M A = ⊤} :=
   sorry -- i have this in a branch
 
 def Theory.lindenbaum [DecidableEq Atom] (T : Theory Atom) : HeytingModel Atom :=
   sorry -- usual Heyting-algebra of propositions modulo equivalence
 
 theorem Theory.lindenbaum_complete [DecidableEq Atom] {T : Theory Atom} :
-    IsCompleteModel (Proposition Atom) (HeytingModel Atom) T T.lindenbaum :=
+    IsCompleteModel (HeytingModel Atom) (Proposition Atom) T T.lindenbaum :=
   sorry -- also in a branch
 
 abbrev Valuation (Atom : Type*) := Atom → Prop
@@ -202,22 +196,21 @@ def Valuation.interp (v : Valuation Atom) : Proposition Atom → Prop
   | .or A B => v.interp A ∨ v.interp B
   | .impl A B => v.interp A → v.interp B
 
-instance : InterpModels (Proposition Atom) (Valuation Atom) where
+instance : HasInterpEntails (Valuation Atom) (Proposition Atom) where
   Ground _ := Prop
   interp v A := v.interp A
   filter _ := {True}
 
 end PL
 
+/-! ### Hindley-Miller logic -/
+
 variable {State Label : Type*}
 
-instance : ParamModels (HML.Proposition Label) (LTS State Label) where
-  Param _ := State
-  SatisfiesAt := HML.Satisfies
+instance : HasEntails  (LTS State Label × State) (HML.Proposition Label) where
+  Entails M := HML.Satisfies M.1 M.2
 
 example (lts : LTS State Label) (s : State) :
-    HML.theory lts s = ParamModels.theory (M := lts) s := by
-  simp [theory, HML.theory]
-  rfl
+  HML.theory lts s = HasEntails.theory (lts, s) := by rfl
 
 end Cslib.Logic
